added all the text cases and the post conditions, need a bit more work

main.dfy
@@ -1,190 +1,451 @@
 
 class {:autocontracts} CarPark {
 
-  const MAX_CAPACITY: int
+  const MAX_CAPACITY: nat
   const MIN_FREE_SPACES := 5
-
+  const reservedCapacity: nat
+  const nonReservedCapacity: nat
+  var isWeekend: bool
   var reservedArea: set<nat>
   var nonReservedArea: set<nat>
-  var reservedCapacity: int
-  var nonReservedCapacity: int
-
-  var nonReservedFreeSpaces: int
-  var reservedFreeSpaces: int
-
-  var isWeekday: bool
   var subscription: set<nat>
 
-  var entryBarrier: bool
+  constructor(maxSize: nat, maxReserved: nat)
+    requires maxSize - 5 >= maxReserved
+    requires maxReserved > 0
 
-
-  constructor(maxSize: nat, maxNonReserved:nat, maxReserved: nat) // Takes a non-negative integer for the carpark spaces
-    requires maxNonReserved > 5
-    requires maxSize == (maxNonReserved + maxReserved)
-
-    ensures isWeekday == true
-    ensures |reservedArea| == 0
-    ensures |nonReservedArea| == 0
+    ensures isWeekend == false
+    ensures reservedArea == nonReservedArea == {}
     ensures |subscription| == 0
+    ensures MAX_CAPACITY == nonReservedCapacity + reservedCapacity
   {
     MAX_CAPACITY := maxSize;
-    nonReservedCapacity := maxNonReserved;
+    nonReservedCapacity := maxSize - maxReserved;
     reservedCapacity := maxReserved;
-
-    isWeekday := true;
-
+    isWeekend := false;
     reservedArea := {};
     nonReservedArea := {};
     subscription := {};
   }
 
-
-  // Function to check the availability of non-reserved spaces
-  // method checkAvailability() returns (available: int)  // to report on the number of non-reserved free spaces currently available
-  // {
-  //   // available;
-  //   // Logic to return the number of non-reserved free spaces currently available
-  //   // Logic to return the number of non-reserved free spaces currently available
-  //   // Do not modify state variables
-  // }
-
-
-  // // Function to close the car park
-  // function closeCarPark(): set<int>
-  // {
-  //     // Logic to return the set of remaining parked cars to be crushed
-  //     // Do not modify state variables
-  // }
-
-  // // Function to get the state invariant
-  // function valid(): bool
-  // {
-  //     // Define the state invariant(s) as a Boolean function
-  //     // Return t+rue when the state invariant(s) hold
-  // }
-
-  // IT just checks the space, otherwise returns false
-  // function isBarrierOpen(): bool
-  // {
-  //   // Implement logic to determine if the barrier is open
-  //   // For simplicity, returning true here, assuming the barrier is always open
-  //   entryBarrier
-  // }
-
   ghost predicate Valid()
-    reads this
   {
-    // 10
-    // First Barrier needs to open for cars as long as it is not full (demed to full when 5 spaces available)
-    |nonReservedArea| < (nonReservedCapacity - 5) 
-    // |nonReservedArea| < (nonReservedCapacity - 5)
-    // true
-    // && (|nonReservedArea| + |reservedArea|) <= MAX_CAPACITY
+    // Rules that must be true throughtout the excution of the program
+    MAX_CAPACITY == (nonReservedCapacity + reservedCapacity)
+    &&
+    MAX_CAPACITY >= (|nonReservedArea| + |reservedArea|)
+    &&
+    |nonReservedArea| <= nonReservedCapacity - MIN_FREE_SPACES // As long as the non-reserved area has the capacity
+    &&
+    |reservedArea| <= reservedCapacity
+    &&
+    |subscription| <= reservedCapacity
+    &&
+
+    // |reservedArea| <= |subscription|
+    // &&
+    nonReservedArea * reservedArea == {} // The same Car must not be in non-reserved or reserved at the same time
+    &&
+    nonReservedArea * subscription == {} // The car must is the nonreservedArea must not be in the subscription
+    // &&
+    // (reservedArea \ subscription == {} )
+    // !(isWeekend && (reservedArea \ subscription != {}))
+
   }
 
+  // To report on the number of non-reserved free spaces currently available
+  method checkAvailability() returns(availablity: nat)
+
+    modifies this
+
+    // Cases
+    ensures !isWeekend ==> (availablity == (nonReservedCapacity - |nonReservedArea|))
+    ensures isWeekend ==> (availablity == (MAX_CAPACITY - (|nonReservedArea| + |reservedArea|)))
+
+    // Preservation of Other State Properties
+    ensures isWeekend == old(isWeekend)
+    ensures nonReservedArea == old(nonReservedArea)
+    ensures reservedArea == old(reservedArea)
+    ensures subscription == old(subscription)
+  {
+    if (isWeekend)
+    {
+      availablity := MAX_CAPACITY - (|nonReservedArea| + |reservedArea|);
+    }
+    else {
+      availablity := nonReservedCapacity - |nonReservedArea|;
+    }
+  }
 
   // To allow any car without a reservation to enter the car park
-  // 
-  // Cars can enter the carpark as long as it is not full, it is full if 5 spaces are left
-  // The system needs  to know how many non-reserved spaces are available
+  method enterCarPark(carID: nat) returns(success: bool)
 
-  method enterCarPark(carID: nat) returns (success: bool)
-    // requires |nonReservedArea| < (nonReservedCapacity - 5)
+    modifies this
 
-    // requires carID !in old(nonReservedArea)
-    // requires ||
-    // requires carID !in nonReservedArea && carID !in reservedArea
-    // requires |nonReservedArea| < MAX_CAPACITY - MIN_FREE_SPACES && |nonReservedArea| < nonReservedCapacity - MIN_FREE_SPACES
-    // requires |nonReservedArea| < nonReservedCapacity - MIN_FREE_SPACES
+    // Good Cases
+    ensures carID !in old(subscription) && carID !in old(nonReservedArea) && (carID !in old(reservedArea))  && (old(|nonReservedArea|) < (nonReservedCapacity - 5)) ==> success
+    ensures success ==> nonReservedArea == old(nonReservedArea) + {carID}
 
-    // modifies this
-    // ensures carID in nonReservedArea || (carID in reservedArea && !isWeekday)
-    // ensures nonReservedArea == old(nonReservedArea) + {carID}
-    // // ensures nonReservedArea == old(nonReservedArea)
-    // ensures subscription == old(subscription)
-    // ensures |nonReservedArea| > 0
-    // ensures isWeekday == old(isWeekday)
+    // Bad Cases
+    ensures carID in old(nonReservedArea) ==> !success
+    ensures carID in old(reservedArea) ==> !success
+    ensures carID in old(subscription) ==> !success
+    ensures old(|nonReservedArea|) >= (nonReservedCapacity - 5) ==> !success
+    ensures !success ==> nonReservedArea == old(nonReservedArea)
 
-    // Car has been added or Car hasn't been added
-    // ensures carID in nonReservedArea  ==> success // Ensures the car has been successfully added in Non-Reserved Area
-    // ensures old(nonReservedArea) != nonReservedArea
-    ensures old(|nonReservedArea|) == (|nonReservedArea| + 1) ==> success && nonReservedArea == old(nonReservedArea) + {carID}
-    // ensures old(|nonReservedArea|) == |nonReservedArea| ==> !success && nonReservedArea == old(nonReservedArea)
-    // ensures old(nonReservedArea) == nonReservedArea + {carID} // Ensures
-    // ensures subscription == old(subscription) // Ensures no changes have been made to subscription
-    // ensures old(|nonReservedArea|) == |nonReservedArea| + 1
+    // Preservation of Other State Properties
+    ensures isWeekend == old(isWeekend)
+    ensures reservedArea == old(reservedArea)
+    ensures subscription == old(subscription)
   {
-    print(|nonReservedArea| < (nonReservedCapacity - 5));
-    // nonReservedArea := nonReservedArea + {carID}; // Adding a car to the non reserved area
-    success := true;
-    // if (|nonReservedArea| < (nonReservedCapacity - 5))
-    // {
-    //   print(|nonReservedArea| < (nonReservedCapacity - 5));
-    //   nonReservedArea := nonReservedArea + {carID}; // Adding a car to the non reserved area
-    //   success := true;
-    // }
-    // else {
-    //   success := false;
-    // }
-
-    // success := false;
+    if ( carID !in nonReservedArea && carID !in reservedArea && carID !in subscription && (|nonReservedArea| < (nonReservedCapacity - 5)))
+    {
+      nonReservedArea := nonReservedArea + {carID};
+      success := true;
+    }
+    else {
+      success := false;
+    }
   }
 
+  // To allow any car from any area to leave the car park
+  method leaveCarPark(carID: nat) returns(left: bool)
+    modifies this
 
+    // Good Cases
+    ensures carID in old(nonReservedArea) ==> left && nonReservedArea == old(nonReservedArea) - {carID}
+    ensures carID in old(reservedArea) ==> left && reservedArea == old(reservedArea) - {carID}
 
+    // Bad Casses - nonReserved/reserved
+    ensures carID !in old(nonReservedArea) && carID !in old(reservedArea) ==> !left
+    ensures !left ==> nonReservedArea == old(nonReservedArea)
+    ensures !left ==> reservedArea == old(reservedArea)
 
-
-
-  // Method to allow any car without a reservation to enter the car park
-  // method enterCarPark()
-  //   modifies NonReservedSpaces
-  //   ensures NonReservedSpaces > 0 && NonReservedSpaces <= Capacity
-  // {
-  //   // Logic to handle entering the car park
-  //   NonReservedSpaces := NonReservedSpaces + 1;
-  // }
-
-
-
-
-  method leaveCarPark() // to allow any car from any area to leave the car park
+    // Preservation of Other State Properties
+    ensures isWeekend == old(isWeekend)
+    ensures subscription == old(subscription)
   {
-    // Logic to allow any car from any area to leave the car park
-    // Update state variables accordingly
+    if (carID in nonReservedArea)
+    {
+      nonReservedArea := nonReservedArea - {carID};
+      left := true;
+    }
+    else if (carID in reservedArea) {
+      reservedArea := reservedArea - {carID};
+      left := true;
+    }
+    else {
+      left := false;
+    }
   }
 
-  method enterReservedCarPark(hasSubscription: bool)
+  // To allow a car with a subscription to enter the car park’s reserved area on a weekday, or to enter the car park generally on a weekend day.
+  method enterReservedCarPark(carID: nat) returns (entered: bool)
+    modifies this
+
+    // Good Cases
+    ensures !isWeekend && carID !in old(nonReservedArea) && carID !in old(reservedArea) && carID in old(subscription) && (old(|reservedArea|)  < reservedCapacity) ==> entered
+    ensures isWeekend && carID !in old(nonReservedArea) && carID !in old(reservedArea) && old(|reservedArea|) < reservedCapacity  ==> entered
+    ensures entered ==> reservedArea == old(reservedArea) + {carID}
+
+    // Bad Cases
+    ensures carID in old(nonReservedArea) ==> !entered
+    ensures carID in old(reservedArea) ==> !entered
+    ensures !isWeekend && carID !in old(subscription) ==> !entered
+    ensures old(|reservedArea|) >= reservedCapacity ==> !entered
+    ensures !entered ==> reservedArea == old(reservedArea)
+
+    // Preservation of Other State Properties
+    ensures isWeekend == old(isWeekend)
+    ensures nonReservedArea == old(nonReservedArea)
+    ensures subscription == old(subscription)
   {
-    // Logic to allow a car with a subscription to enter the reserved area on a weekday
-    // or to enter the car park generally on a weekend day
-    // Update state variables accordingly
+    if (!isWeekend && carID in subscription && carID !in reservedArea && carID !in nonReservedArea && |reservedArea| < reservedCapacity)
+    {
+      reservedArea := reservedArea + {carID};
+      entered := true;
+    }
+    else if (isWeekend && carID !in reservedArea && carID !in nonReservedArea && |reservedArea| < reservedCapacity)
+    {
+      reservedArea := reservedArea + {carID};
+      entered := true;
+    }
+    else {
+      entered := false;
+    }
   }
 
-  method makeSubscription(carID: int)
+  // // Logic to allow a car to be registered as having a reserved space when the owner pays the subscription
+  method makeSubscription(carID: nat) returns(registered: bool)
+    // requires |subscription| < |reservedArea|
+    modifies this
+
+    // Good Cases
+    ensures carID !in old(subscription) && carID !in old(nonReservedArea) && carID !in old(reservedArea) && old(|subscription|) < reservedCapacity ==> registered
+    ensures registered ==> subscription == old(subscription) + {carID}
+
+    // Bad Cases
+    ensures carID in old(subscription) ==> !registered
+    ensures carID in old(nonReservedArea) ==> !registered
+    ensures carID in old(reservedArea) ==> !registered
+    ensures old(|subscription|) >= reservedCapacity ==> !registered
+    ensures !registered ==> subscription == old(subscription)
+
+    // Preservation of Other State Properties
+    ensures isWeekend == old(isWeekend)
+    ensures nonReservedArea == old(nonReservedArea)
+    ensures reservedArea == old(reservedArea)
   {
-    // Logic to allow a car to be registered as having a reserved space when the owner pays the subscription
-    // as long as subscriptions are available
-    // Update state variables accordingly
+    if ( carID !in subscription && carID !in nonReservedArea && carID !in reservedArea && |subscription| < reservedCapacity)
+    {
+      subscription := subscription + {carID};
+      registered := true;
+    }
+    else{
+      registered := false;
+    }
   }
 
-  method openReservedArea()
+  // To remove parking restrictions on the reserved spaces (at the weekend).
+  method openReservedArea() returns (open: bool)
+    modifies this
+
+    // Good Cases
+    ensures old(isWeekend) == false ==> open
+    ensures open ==> isWeekend == true
+
+    //Bad Cases
+    ensures old(isWeekend) == true ==> !open
+    ensures !open ==> old(isWeekend) == isWeekend
+
+    // Preservation of Other State Properties
+    ensures nonReservedArea == old(nonReservedArea)
+    ensures reservedArea == old(reservedArea)
+    ensures subscription == old(subscription)
   {
-    // Logic to remove parking restrictions on the reserved spaces during the weekend
-    // Update state variables accordingly
+    if (isWeekend == false)
+    {
+      isWeekend := true;
+      open := true;
+    }
+    else {
+      open := false;
+    }
   }
 
+  // To remove and crush remaining parked cars at closing time
+  method closeCarPark()
+    modifies this
 
+    // Good Cases
+    ensures nonReservedArea == {}
+    ensures reservedArea == {}
+    ensures isWeekend == false
 
+    // Preservation of Other State Properties
+    ensures subscription == old(subscription)
+  {
+    nonReservedArea := {};
+    reservedArea := {};
+    isWeekend := false;
+  }
+
+  method PrintBasicPlan()
+  {
+    print("\nCarPark Max Capacity: ");
+    print(MAX_CAPACITY);
+    print("\n");
+    print("Non Reserved Max Capacity: ");
+    print(nonReservedCapacity);
+    print("\n");
+    print("Reserved Max Capacity: ");
+    print(reservedCapacity);
+    print("\n-----------------------------");
+  }
+
+  method PrintParkingPlan()
+  {
+    // var nonReservedSpace := checkAvailability();
+    print("Current CarPark Status");
+    print("\n>Non-Reserved Area: ");
+    print(nonReservedArea);
+    // print("   Spaces Left[");
+    // print(nonReservedSpace);
+    // print("]");
+    print("\n");
+    print(">Reserved Area: ");
+    print(reservedArea);
+    print("\n");
+    print(">Current Subscriptions: ");
+    print(subscription);
+    // print("\n");
+  }
 }
-
 
 method Main()
 {
-  var fullCarParkCapacity := 11;
-  var nonReservedCarParkCapacity := 6;
+  // NOTE: PLEASE UNCOMMENT EACH FUNCTION TESTCASES, OTHERWISE VSCODE CAN timeout
+  var fullCarParkCapacity := 13;
   var reservedCarParkCapacity := 5;
+  var cp: CarPark := new CarPark( fullCarParkCapacity, reservedCarParkCapacity);
 
-  var cp: CarPark := new CarPark(fullCarParkCapacity, nonReservedCarParkCapacity, reservedCarParkCapacity);
-  var a := cp.enterCarPark(5);
-  // var b := cp.enterCarPark(10);
+  print("====================================\n");
+  print("               CarPark              \n");
+  print("====================================");
+  cp.PrintBasicPlan();
+
+  ////////////// Testing the enterCarPark()
+  ////// Testing if the car can enter the non-reserved area
+  print("\nTEST 1 \n");
+  var carID1 := cp.enterCarPark(5);
+  print("-carID1(5) has entered the Non-Reserved Area: ");
+  print(carID1);
+  print("\n-----------------------------\n");
+
+
+  ////// Testing if the same car can enter the carpark twice
+  print("TEST 2 \n");
+  var carID1Duplicate := cp.enterCarPark(5);
+  print("-carID1(5) has entered the Non-Reserved Area: ");
+  print(carID1Duplicate);
+  print(" (fails as the same car tries to enter again)");
+  print("\n-----------------------------\n");
+
+  ////// Testing if the non-reserved are is deemed to be full when 5 spaces are left
+  print("TEST 3 \n");
+  var carID2 := cp.enterCarPark(12);
+  var carID3 := cp.enterCarPark(19);
+  var carID4 := cp.enterCarPark(21);
+  print("-carID2(12) has entered the Non-Reserved Area: ");
+  print(carID2);
+  print("\n");
+  print("-carID3(19) has entered the Non-Reserved Area: ");
+  print(carID3);
+  print("\n");
+  print("-carID4(21) has entered the Non-Reserved Area: ");
+  print(carID4);
+  print(" (fails because only 5 spaces are left in the non-reserved area)");
+  // print("\n");
+  print("\n-----------------------------\n");
+
+  ////// Testing if the car with subscription can enter the non-reserved carpark -- CONFIRMED
+  print("TEST 4\n");
+  //Making two cars leave to make a space in the carpark
+  var carID3Leaving := cp.leaveCarPark(19);
+  var carID4Leaving := cp.leaveCarPark(19);
+
+  // Making a subscription for the car
+  var carID5Subscription := cp.makeSubscription(9);
+  print("-carID5(9) has registered as having a reserved space: ");
+  print(carID5Subscription);
+  print("\n");
+
+  var carID5 := cp.enterCarPark(9);
+  print("-carID5(9) has entered the Non-Reserved Area: ");
+  print(carID5);
+  print(" (fails to enter because it has a subscription-reserved Space)");
+  print("\n-----------------------------\n");
+
+  cp.PrintParkingPlan();
+  print("\n-----------------------------\n");
+
+
+
+
+  ////////////// Testing the leaveCarPark()
+  ////// Testing if a car not parked in the park can leave
+  print("TEST 5\n");
+  var carID5Left := cp.leaveCarPark(9);
+  print("-carID5(9) has left the carPark: ");
+  print(carID5Left);
+  print(" (fails to leave as their is no carID5(9) car in the carpark)");
+  print("\n");
+  print("\n-----------------------------\n");
+
+  ////// Testing if a car parked in a non-reserved area can leave
+  print("TEST 6\n");
+  var carID2Left := cp.leaveCarPark(12);
+  print("-carID2(12) has left the carpark(Non-Reserved Area): ");
+  print(carID2Left);
+  print("\n-----------------------------\n");
+
+  ////// Testing if a car parked in a reserved area can leave
+  print("TEST 7\n");
+  var carID6 := cp.enterReservedCarPark(9);
+  print("-carID6(9) has entered the Non-Reserved Area: ");
+  print(carID6);
+  print("\n-----------------------------\n");
+
+  ////////////// Testing the checkAvailability() 
+  ////// Testing if the availability status is correct on Weekday -- MAYNEEDSOMEWORK
+  print("TEST 8\n");
+  var nonReservedAvailability := cp.checkAvailability();
+  print("Current Non-Reserved Area Availability (on Weekday): ");
+  print(nonReservedAvailability);
+  print("\n-----------------------------\n");
+
+  ////////////// Testing the makeSubscription()
+  ////// Testing if it can make a subscription twice for the same car
+  print("TEST 9\n");
+  var carID6Subscription := cp.makeSubscription(9);
+  print("-carID6(9) has registered as having a reserved space: ");
+  print(carID6Subscription);
+  print(" (fails to make a subscription, because it already has a subscription)");
+  print("\n-----------------------------\n");
+
+  ////// Testing if it can make a subscription for car already parked in non-reserved area -- CONFIRMED
+  print("TEST 10\n");
+  var carID1Subscription := cp.makeSubscription(5);
+  print("-carID1(5) has registered as having a reserved space: ");
+  print(carID1Subscription);
+  print(" (fails to make a subscription, because it is already parked in Non-Reserved Area)");
+  print("\n-----------------------------\n");
+
+
+
+
+  ////////////// Testing the enterReservedCarPark()
+  ////// Testing if car without a subscription can enter the reserved area.
+  print("TEST 11\n");
+  var carID7 := cp.enterReservedCarPark(231);
+  print("-carID7(231) has entered the Reserved Area: ");
+  print(carID7);
+  print(" (fails to enter because doesn't have subscription)");
+  print("\n-----------------------------\n");
+
+  ////// Testing if car is already parked in a reserved can enter again
+  print("TEST 12\n");
+  var carID8 := cp.enterReservedCarPark(9);
+  var carID8Duplicate := cp.enterReservedCarPark(9);
+  print("-carID8(9) has entered the Reserved Area: ");
+  print(carID8Duplicate);
+  print(" (fails because same car can't enter again)");
+  print("\n-----------------------------\n");
+
+  ////// Testing if a car without the subscription can enter the reserved area on weekend -- NEEDSOMEWORK
+  print("TEST 13\n");
+  var isReservedOpen := cp.openReservedArea();
+  var carID9 := cp.enterReservedCarPark(98);
+  print("-carID9(98) has entered the Reserved Area: ");
+  print(carID9);
+  print(" (enters without making a subscription, because it is a Weekend!)");
+  print("\n-----------------------------\n");
+
+  ////////////// Testing the openReservedArea()
+  ////// Testing if it can open reserved area if it already opened -- NEEDSOMEWORK
+  print("TEST 14\n");
+  var alreadyOpened := cp.openReservedArea();
+  print("Reserved Area is opened: ");
+  print(alreadyOpened);
+  print(" (fails to open, because it is already opened)");
+  print("\n-----------------------------\n");
+
+
+  ////////////// Testing the closeCarPark()
+  ////// Testing if all the cars are removed when the function is called
+  print("TEST 15\n");
+  cp.closeCarPark();
+  print("The carPark has been closed!");
+  cp.PrintParkingPlan();
+  print("\n-----------------------------\n");
 }
